kalloc/Spec_kalloc.v
@@ -4,6 +4,7 @@ Require Import VC.ASI_kalloc.
 Require Import VC.kalloc.
 Require Import VC.kallocfun.
 Require Import VC.kalloc_kfree_definitions.
+Require Import VC.tactics.
 
 Global Open Scope funspec_scope.
 
@@ -11,7 +12,7 @@ Global Open Scope funspec_scope.
 (******************************)
 
 (*** kalloc token type... *)
-Definition my_kalloc_token K {cs: compspecs} sh t p :=
+Definition my_kalloc_token {cs: compspecs} K sh t p :=
   !! field_compatible t [] p && (* this should work because of memory_block_data_at_*)
   (kalloc_token' K sh (sizeof t) p).
 
@@ -20,7 +21,9 @@ Lemma my_kalloc_token_valid_pointer:
   my_kalloc_token K sh t p |-- valid_pointer p.
 Proof.
   intros. 
-  unfold my_kalloc_token. unfold kalloc_token_sz. entailer!.
+  unfold my_kalloc_token. apply andp_left2.
+  sep_apply kalloc_token'_local_facts.
+  entailer!.
 Qed.
 
 Ltac kalloc_token_data_at_valid_pointer :=
@@ -46,12 +49,17 @@ Ltac kalloc_token_data_at_valid_pointer :=
 #[export] Hint Extern 4 (_ |-- valid_pointer _) => kalloc_token_data_at_valid_pointer : valid_pointer.
 
 Lemma my_kalloc_token_local_facts: forall K {cs: compspecs} sh t p,
-      my_kalloc_token K sh t p |-- !! (field_compatible t [] p /\ malloc_compatible (sizeof t) p).
+      my_kalloc_token K sh t p |-- !! (field_compatible t [] p /\ (
+        0 < sizeof t <= PGSIZE
+        /\ malloc_compatible (sizeof t) p 
+        /\ malloc_compatible (PGSIZE) p
+        /\ writable_share sh
+        /\ malloc_compatible (sizeof t) p)).
 Proof. intros.
  unfold my_kalloc_token.
  normalize. rewrite prop_and.
  apply andp_right. apply prop_right; auto.
- apply kalloc_token'_local_facts.
+ sep_apply kalloc_token'_local_facts. entailer!.
 Qed.
 #[export] Hint Resolve my_kalloc_token_local_facts : saturate_local.
 
@@ -65,9 +73,43 @@ Lemma my_kalloc_token_split:
 Proof.
   intros. apply pred_ext.
   - unfold my_kalloc_token. entailer.
-  - unfold my_kalloc_token. entailer!.
+  - unfold my_kalloc_token. apply andp_right.
+    + apply andp_left1. entailer.
+    + apply andp_left2. apply derives_refl.
 Qed.
 
+Fixpoint my_kalloc_tokens (K:KallocFreeAPD) (sh: share) (n: nat) (p: val) (size: Z) (t:type): mpred :=
+  match n with
+  | S n' => 
+      (sepcon
+      (my_kalloc_token K sh t p)
+      (my_kalloc_tokens K sh n' (offset_val size p) size t)) (* Move to the next slot *)
+  | O => !! (p = nullval) && emp
+  end.
+
+Definition my_kalloc_tokens_range K (sh: share) (p_start p_end: val) (size: Z) :=
+    match p_start, p_end with
+    | Vptr b_s p_s, Vptr b_e p_e =>
+      if (sameblock p_start p_end) then
+        my_kalloc_tokens K sh (Z.to_nat (compute_c p_start p_end size)) p_start size
+      else !! (p_start = nullval) && emp
+    | _ , _ => !! (p_start = nullval) && emp
+    end.
+
+Arguments my_kalloc_tokens_range K sh p_start p_end size : simpl never.
+
+Lemma my_kalloc_tokens_local_prop: forall K sh n p size t, 
+  my_kalloc_tokens K sh n p size t |--  !! (is_pointer_or_null p /\ (n=0<->p=nullval) /\ (n>0<->isptr p))%nat.
+Proof.
+  intros K sh n.
+  induction n as [| n' IH].
+  - unfold my_kalloc_tokens. entailer!. split; split; intros; auto; auto_contradict; try rep_lia.
+  - unfold my_kalloc_tokens; fold my_kalloc_tokens. intros. sep_apply IH. entailer!. destruct p; auto_contradict.
+  split; split; intros; try rep_lia; auto; auto_contradict.
+Qed.
+#[export] Hint Resolve kalloc_tokens_local_prop : saturate_local.
+
+(************************ specs *********************)
 
 Definition kfree_spec (K:KallocFreeAPD) {cs: compspecs} (t: type) := 
   DECLARE _kfree
@@ -117,7 +159,33 @@ POST [ tptr tvoid ]
         )
     ).
 
+Definition kfree_loop_spec (K:KallocFreeAPD) {cs: compspecs} (t: type) := 
+  DECLARE _kfree_loop
+  WITH sh : share, pa1:val, original_freelist_pointer:val, xx:Z, gv:globals, ls : list val, n:Z
+  PRE [ tptr tvoid, tint ]
+      PROP(
+          isptr pa1 /\
+          Int.min_signed <= Int.signed (Int.repr n) + Int.signed (Int.repr 1) <= Int.max_signed /\
+          0 <= n <= Int.max_signed
+      ) 
+      PARAMS (pa1; Vint (Int.repr n)) GLOBALS(gv)
+      SEP (
+          my_kalloc_tokens K sh (Z.to_nat n)%nat pa1 PGSIZE t *
+          ASI_kalloc.mem_mgr K gv sh ls xx original_freelist_pointer
+      )
+  POST [ tvoid ]
+      EX head, EX added_elem, (* TODO: fix top and next is the same?? *)
+      PROP( 
+          added_elem = (pointers_with_original_head (Z.to_nat n) (pa1) PGSIZE original_freelist_pointer) /\
+          head = (hd nullval ((pointers_with_original_head (Z.to_nat n+1) (pa1) PGSIZE original_freelist_pointer)++ls))
+          )
+          RETURN () (* we return the head like in the pop function*)
+          SEP 
+          (
+            ASI_kalloc.mem_mgr K gv sh (added_elem++ls) xx head
+          ).
 
+(************** convert to size version ***************)
 
 Lemma kalloc_spec_sub:
   forall  (K:KallocFreeAPD) {cs: compspecs} (t: type), 
@@ -143,11 +211,10 @@ forall  (K:KallocFreeAPD) {cs: compspecs} (t: type),
   funspec_sub (snd (kfree_spec' K _kfree)) (snd (kfree_spec K t)).
 Proof.
   do_funspec_sub. 
-  destruct w.
-  repeat (destruct p).
-  Exists (sizeof t, v0, g0, s, l, z, v) emp.
+  destruct w as [[[[[new_head gv] sh] ls] xx] original_freelist_pointer].
+  Exists (sizeof t, new_head, gv, sh, ls, xx, original_freelist_pointer) emp.
   entailer!.
-  destruct (EqDec_val v0 nullval) eqn:Heq; entailer.
+  destruct (EqDec_val new_head nullval) eqn:Heq; entailer.
   unfold my_kalloc_token. entailer.
 Qed.
 
@@ -157,3 +224,57 @@ Ltac simplify_kalloc_token :=
     unfold my_kalloc_token
   );
   entailer!.
+
+Lemma my_kalloc_tokens_entails_kalloc_tokens_sz:
+  forall n K sh pa1 t,
+    my_kalloc_tokens K sh (Z.to_nat n) pa1 PGSIZE t
+    |-- kalloc_tokens_sz sh (sizeof t) pa1 PGSIZE (Z.to_nat n).
+Proof.
+  intros n.
+  induction (Z.to_nat n).
+  - intros. 
+  unfold my_kalloc_tokens, kalloc_tokens_sz. entailer.
+  - intros. unfold my_kalloc_tokens, kalloc_tokens_sz. 
+  fold my_kalloc_tokens; fold kalloc_tokens_sz.
+  sep_apply IHn0. entailer!. unfold my_kalloc_token.
+  apply andp_left2.
+  sep_apply kalloc_token'_local_facts. unfold kalloc_token_sz. entailer!. 
+Qed.
+
+
+Lemma kfree_loop_spec_sub:
+forall  (K:KallocFreeAPD) {cs: compspecs} (t: type), 
+  funspec_sub (snd (kfree_loop_spec' K)) (snd (kfree_loop_spec K t)).
+Proof.
+  do_funspec_sub.
+  destruct w as [[[[[[sh pa1] original_freelist_pointer] xx] gv] ls] n].
+  Exists (sh, pa1, original_freelist_pointer, xx, gv, ls, n, sizeof t, PGSIZE) emp.
+  entailer!.
+  -intros tau ?.
+  Exists (hd nullval
+            (pointers_with_original_head (Z.to_nat n + 1) pa1 PGSIZE original_freelist_pointer ++
+            ls))
+          (pointers_with_original_head (Z.to_nat n) pa1 PGSIZE original_freelist_pointer).
+          entailer!.
+          assert (kallocfun.PGSIZE = PGSIZE). { unfold kallocfun.PGSIZE, PGSIZE; auto. }
+          apply derives_refl.
+    - sep_apply my_kalloc_tokens_entails_kalloc_tokens_sz. entailer!. apply derives_refl.
+    
+    generalize dependent pa1. induction (Z.to_nat n).
+      + unfold my_kalloc_tokens, kalloc_tokens_sz. intros. entailer!.
+      + intros. unfold my_kalloc_tokens, kalloc_tokens_sz. fold my_kalloc_tokens; fold kalloc_tokens_sz. 
+        sep_apply IHn0; auto. 
+        sep_apply my_kalloc_tokens_entails_kalloc_tokens_sz.
+
+  rewrite mem_mgr_split.
+  unfold my_kalloc_tokens.
+  Exists (s, v0, g0, s, l, z, v) emp.
+  (*Exists (sizeof t, v0, g0, s, l, z, v) emp.*)
+  entailer!.
+  destruct (EqDec_val v0 nullval) eqn:Heq; entailer.
+  unfold my_kalloc_token. entailer.
+Qed.
+
+
+
+
