kalloc/kalloc_kfree_definitions.v
@@ -26,7 +26,12 @@ Qed.
 
 Lemma  kalloc_token_sz_local_facts : 
  forall (sh : share) (n:Z) (p : val) ,
-   kalloc_token_sz sh n p |-- !! malloc_compatible n p.
+   kalloc_token_sz sh n p |-- (!! (
+    0 < n <= PGSIZE
+    /\ malloc_compatible (n) p 
+    /\ malloc_compatible (PGSIZE) p
+    /\ writable_share sh
+    /\ malloc_compatible n p) && memory_block sh (n) (p)).
 Proof.
   intros. 
   unfold kalloc_token_sz. simpl. entailer.
@@ -47,6 +52,66 @@ Proof.
   - unfold kalloc_token_sz. entailer.
   - unfold kalloc_token_sz. entailer!.
 Qed.
+
+Fixpoint  kalloc_tokens_sz (sh: share) (type_sz: Z) (p: val) (pgsize: Z) (n:nat): mpred :=
+  match n with
+  | S n' => 
+      sepcon
+      (kalloc_token_sz sh type_sz p)
+      (kalloc_tokens_sz sh type_sz (offset_val pgsize p) pgsize n') (* Move to the next slot *)
+  | O => !! (p = nullval) && emp
+  end.
+
+Definition  kalloc_tokens_sz_range (sh: share) (type_sz:Z) (p_start p_end: val) (pgsize: Z) := (* size is pgsize, sz is size of token*)
+    match p_start, p_end with
+    | Vptr b_s p_s, Vptr b_e p_e =>
+      if (sameblock p_start p_end) then
+         kalloc_tokens_sz sh type_sz p_start pgsize (Z.to_nat (compute_c p_start p_end pgsize))
+      else !! (p_start = nullval) && emp
+    | _ , _ => !! (p_start = nullval) && emp
+    end.
+
+Arguments  kalloc_tokens_sz_range sh type_sz p_start p_end pgsize : simpl never.
+
+Lemma  kalloc_tokens_sz_local_prop: forall sh type_sz n p pgsize, 
+   kalloc_tokens_sz sh type_sz p pgsize n |--  !! (is_pointer_or_null p /\ (n=0<->p=nullval) /\ (n>0<->isptr p))%nat.
+Proof.
+  intros.
+  generalize dependent p.
+  induction n as [| n' IH].
+  - unfold  kalloc_tokens_sz. entailer!. split; split; intros; auto; auto_contradict; try rep_lia.
+  - unfold  kalloc_tokens_sz; fold  kalloc_tokens_sz. intros. sep_apply IH. entailer!. destruct p; auto_contradict.
+  split; split; intros; try rep_lia; auto; auto_contradict.
+  + split; intros; auto_contradict.
+  + split; intros; auto; rep_lia.
+Qed.
+#[export] Hint Resolve  kalloc_tokens_sz_local_prop : saturate_local.
+
+Definition kfree_loop_spec' (K:KallocFreeAPD) {cs: compspecs} := 
+  DECLARE _kfree_loop
+  WITH sh : share, pa1:val, original_freelist_pointer:val, xx:Z, gv:globals, ls : list val, n:Z, type_sz:Z, pgsize:Z
+  PRE [ tptr tvoid, tint ]
+      PROP(
+          isptr pa1 /\
+          Int.min_signed <= Int.signed (Int.repr n) + Int.signed (Int.repr 1) <= Int.max_signed /\
+          0 <= n <= Int.max_signed
+      ) 
+      PARAMS (pa1; Vint (Int.repr n)) GLOBALS(gv)
+      SEP (
+           kalloc_tokens_sz sh type_sz pa1 pgsize (Z.to_nat n)%nat *
+          ASI_kalloc.mem_mgr K gv sh ls xx original_freelist_pointer
+      )
+  POST [ tvoid ]
+      EX head, EX added_elem, (* TODO: fix top and next is the same?? *)
+      PROP( 
+          added_elem = (pointers_with_original_head (Z.to_nat n) (pa1) PGSIZE original_freelist_pointer) /\
+          head = (hd nullval ((pointers_with_original_head (Z.to_nat n+1) (pa1) PGSIZE original_freelist_pointer)++ls))
+          )
+          RETURN () (* we return the head like in the pop function*)
+          SEP 
+          (
+            ASI_kalloc.mem_mgr K gv sh (added_elem++ls) xx head
+          ).
 
 (***** kalloc token size ******)
 
@@ -81,7 +146,6 @@ Proof.
 Qed.
 
 (************ lemmas etc. end *************)
-
 
 Definition KF_APD := Build_KallocFreeAPD Tok_APD mem_mgr.
 
